

Adam's amazing formula

$$(a+b)^2 = a^2 + 2ab + b^2$$

$$ax^2 + bx + c = y$$

$$x^2 + \frac{b}{a}x + \frac{c}{a} = \frac{y}{a}$$

$$x^2 + \frac{b}{a}x = \frac{y}{a} - \frac{c}{a}$$

$$x^2 + \frac{b}{a}x + \left(\frac{b}{2a}\right)^2 = \frac{y-c}{a} + \left(\frac{b}{2a}\right)^2$$

$$\left(x + \frac{b}{2a}\right)^2 = \frac{y-c}{a} + \frac{b^2}{4a^2}$$

$$a\left(x + \frac{b}{2a}\right)^2 = y - c + \frac{b^2}{4a}$$

let k be
a shift

$$a\left(x + \frac{b}{2a}\right)^2 + c - \frac{b^2}{4a} = y$$

$$a\left(x + \frac{b}{2a} - k\right)^2 + c - \frac{b^2}{4a} = y$$

↳
Simp.

$$ak^2 - 2akx + ax^2 - bk + bx + c = y$$

⇓

$$ax^2 + \underbrace{2ak}_{\downarrow}x + \underbrace{ak^2 - bk + bx + c}_{\downarrow}$$

$$\downarrow \quad \downarrow \quad \downarrow$$
$$ax^2 + bx + c \leftarrow$$